\documentclass{article}
\usepackage[utf8]{inputenc}
\usepackage[margin=1in]{geometry}
\usepackage[utf8]{inputenc}
\usepackage{amsmath,amssymb}
\usepackage{listings}
\usepackage{color}
\usepackage[]{graphicx}

\renewcommand*\rmdefault{iwona}

\title{Geometric Flows}
\author{Orton Babb, Aneesh Malhotra, Ryan Vaughan}
\date{Fall 2017}

\begin{document}

\maketitle

\section{Constructing the Normalized Graph Laplacian on a Manifold}

\section{Heat Flow}

Suppose $\frac{\partial}{\partial t} \tilde{f} = - \Delta \tilde{f}$ with $\tilde{f}(0, \theta) = f_0(\theta)$. Note that if $\tilde{f}$ is an eigenfunction of $\Delta$, then $\Delta\tilde{f}=\lambda \tilde{f}$. Since $\frac{\partial}{\partial t} \tilde{f} = - \lambda \tilde{f}$, this has the solution $\tilde{f}(t, \theta) = e^{-\lambda t}f_0 (\theta)$. More generally, we want to expand $\tilde{f}$ to its generalized fourier series:
$$ \tilde{f}(t,\theta) = \sum_{n=0}^{\infty} c_n(t)\phi_n(\theta)$$

Let $\phi$, so that  $\Delta \phi_n = \lambda_n \phi_n $, be the eigenfunctions of $\Delta$. Then,

\begin{align*}
\frac{\partial}{\partial t} \tilde{f} &= \sum_{n=0}^{\infty} \dot{c}_n(t)\phi_n(\theta) &= \Delta \tilde{f} &= \sum_{n=0}^{\infty} c_n(t) \Delta \phi_n(\theta) \\
%&= \sum_{n=0}^{\infty} c_n(t) \lambda_n \phi_n(\theta)
\end{align*}

\end{document}
